libcrux-ml-dsa/proofs/fstar/extraction/RmMe.fst
@@ -3,40 +3,100 @@ module RmMe
 open Core
 open FStar.Mul
 
-module BV_LEMMAS = Core_models.Abstractions.Bitvec.Int_vec_interp
+open Libcrux_ml_dsa.Simd.Avx2.Arithmetic
+open FStar.FunctionalExtensionality    
+
+// open Core_models.Core_arch.X86.Interpretations.Int_vec.Lemmas
+open Core_models.Abstractions.Bitvec.Int_vec_interp
+
+unfold let i = mk_u64 0
+
+// ///Lemma that asserts that applying BitVec :: < 256 > :: from and then i32x8 :: from is the identity.
+// assume
+// val e_ee_1__lemma_cancel_iv' (x: Core_models.Abstractions.Funarr.t_FunArray (mk_u64 8) i32)
+
+//   : Lemma
+//       (ensures
+//         (e_ee_1__impl__to_i32x8 (e_ee_1__impl__from_i32x8 x)) ==
+//         x)
+//       [SMTPat (e_ee_1__impl__to_i32x8 (e_ee_1__impl__from_i32x8 x))]
 
 
-///Lemma that asserts that applying BitVec :: < 256 > :: from and then i32x8 :: from is the identity.
-let e_ee_1__lemma_cancel_iv'
-  (x: Core_models.Abstractions.Funarr.t_FunArray (mk_u64 8) i32) 
-  arg
-  : Lemma
-      (ensures
-        (BV_LEMMAS.e_ee_1__impl__to_i32x8 (BV_LEMMAS.e_ee_1__impl__from_i32x8 x
-              <:
-              Core_models.Abstractions.Bitvec.t_BitVec (mk_u64 256))
-          <:
-          Core_models.Abstractions.Funarr.t_FunArray (mk_u64 8) i32) arg ==
-        x arg)
-      [
-        SMTPat
-        ((BV_LEMMAS.e_ee_1__impl__to_i32x8 (BV_LEMMAS.e_ee_1__impl__from_i32x8 x
-              <:
-              Core_models.Abstractions.Bitvec.t_BitVec (mk_u64 256))
-          <:
-          Core_models.Abstractions.Funarr.t_FunArray (mk_u64 8) i32) arg)
-      ]
-      = admit ()
+// ///Lemma that asserts that applying i32x8 :: from and then BitVec :: < 256 > :: from is the identity.
+// assume
+// val e_ee_1__lemma_cancel_bv': x: Core_models.Abstractions.Bitvec.t_BitVec (mk_u64 256)
+//   -> Lemma
+//       (ensures
+//         (e_ee_1__impl__from_i32x8 (e_ee_1__impl__to_i32x8 x)) == x)
+//       [
+//         SMTPat (e_ee_1__impl__from_i32x8 (e_ee_1__impl__to_i32x8 x))
+//       ]
 
 
-let hey lhs rhs: squash (
-        Core_models.Abstractions.Bitvec.Int_vec_interp.e_ee_1__impl__to_i32x8 (montgomery_multiply lhs rhs) (mk_u64 0)
-     == montgomery_multiply_spec 
-          (Core_models.Abstractions.Bitvec.Int_vec_interp.e_ee_1__impl__to_i32x8 lhs (mk_u64 0)) 
-          (Core_models.Abstractions.Bitvec.Int_vec_interp.e_ee_1__impl__to_i32x8 rhs (mk_u64 0))
-    ) = _ by (
-      let open FStar.Tactics in
-      norm [iota; primops; delta_only [`%montgomery_multiply]; zeta];
-      l_to_r [`e_ee_1__lemma_cancel_iv'];
-      dump "goal"
+// ///Lemma that asserts that applying i32x8 :: from and then BitVec :: < 256 > :: from is the identity.
+// assume
+// val e_ee_1__lemma_cancel_bv'2: x: Core_models.Abstractions.Bitvec.t_BitVec (mk_u64 256) -> i:(i:u64 {v i < 8})
+//   -> Lemma
+//       (ensures (e_ee_1__impl__from_i32x8 (e_ee_1__impl__to_i32x8 x)).[i] == x.[i])
+//       [SMTPat (((e_ee_1__impl__from_i32x8 (e_ee_1__impl__to_i32x8 x)).[i]))]
+
+open FStar.Tactics
+
+let lemma lhs rhs (i: u64 {v i < 8}): squash (
+     (e_ee_1__impl__to_i32x8 (montgomery_multiply lhs rhs)).[i]
+  == (montgomery_multiply_spec
+        ((e_ee_1__impl__to_i32x8 lhs).[i])
+        ((e_ee_1__impl__to_i32x8 rhs).[i])
     )
+) = _ by (
+  norm [iota; primops; delta_only [`%montgomery_multiply]; zeta];
+  l_to_r [`Core_models.Abstractions.Bitvec.Int_vec_interp.e_ee_1__lemma_cancel_iv]
+)
+
+// type fnarr (n: u64) (t: Type0) = i:u64 {v i < v n} ^-> t
+// assume val bv: Type0
+
+// assume val from_i32x8: fnarr (mk_u64 8) i32 -> bv
+// assume val to_i32x8: bv -> fnarr (mk_u64 8) i32
+
+
+// let to_from_i32x8 (x: fnarr (mk_u64 8) i32) (i: u64 {v i < 8})
+//   : Lemma (to_i32x8 (from_i32x8 x) i == x i) [SMTPat (to_i32x8 (from_i32x8 x) i)]
+//       = admit ()
+
+// let to_from_i32x8' (x: fnarr (mk_u64 8) i32)
+//   : Lemma (to_i32x8 (from_i32x8 x) == x) [SMTPat (to_i32x8 (from_i32x8 x))]
+//       = admit ()
+
+// assume val spec: i32 -> i32 -> i32
+
+// module RI = Rust_primitives.Integers
+
+// let body (lhs rhs: bv): fnarr (mk_u64 8)  =
+//   (FStar.FunctionalExtensionality.on_domain (i:
+//         RI.u64 { RI.v i < RI.v (RI.mk_u64 8) })
+//       (fun i ->
+//           match i with
+//           | RI.MkInt 0 -> spec (to_i32x8 lhs (RI.mk_u64 0)) (to_i32x8 rhs (RI.mk_u64 0))
+//           | RI.MkInt 1 -> spec (to_i32x8 lhs (RI.mk_u64 1)) (to_i32x8 rhs (RI.mk_u64 1))
+//           | RI.MkInt 2 -> spec (to_i32x8 lhs (RI.mk_u64 2)) (to_i32x8 rhs (RI.mk_u64 2))
+//           | RI.MkInt 3 -> spec (to_i32x8 lhs (RI.mk_u64 3)) (to_i32x8 rhs (RI.mk_u64 3))
+//           | RI.MkInt 4 -> spec (to_i32x8 lhs (RI.mk_u64 4)) (to_i32x8 rhs (RI.mk_u64 4))
+//           | RI.MkInt 5 -> spec (to_i32x8 lhs (RI.mk_u64 5)) (to_i32x8 rhs (RI.mk_u64 5))
+//           | RI.MkInt 6 -> spec (to_i32x8 lhs (RI.mk_u64 6)) (to_i32x8 rhs (RI.mk_u64 6))
+//           | RI.MkInt 7 -> spec (to_i32x8 lhs (RI.mk_u64 7)) (to_i32x8 rhs (RI.mk_u64 7))))
+
+// let test (lhs rhs: bv) = from_i32x8 (body lhs rhs)
+
+// let test_lemma (lhs rhs: bv) =
+//     // to_from_i32x8 (body lhs rhs) (mk_u64 0);
+//     assert (
+//         to_i32x8 (test lhs rhs) (mk_u64 0)
+//      == spec (to_i32x8 lhs (mk_u64 0)) (to_i32x8 rhs (mk_u64 0))
+//     ) 
+//     // by (
+//     //   let open FStar.Tactics in
+//     //   norm [iota; primops; delta_only [`%test]; zeta];
+//     //   // l_to_r [`e_ee_1__lemma_cancel_iv'];
+//     //   dump "goal"
+//     // )
