libcrux-ml-dsa/proofs/fstar/extraction/RmMe2.fst
@@ -1,0 +1,46 @@
+module RmMe2
+#set-options "--fuel 0 --ifuel 1 --z3rlimit 80"
+
+open FStar.Mul
+open FStar.FunctionalExtensionality
+
+unfold type fnarr (n: nat) (t: Type0) = i:nat {i < n} ^-> t
+
+assume val i32: Type0
+
+assume val bv: Type0
+assume val from_i32x8: fnarr 8 i32 -> bv
+assume val to_i32x8: bv -> fnarr 8 i32
+
+let to_from_i32x8 (x: fnarr 8 i32) (i: nat {i < 8})
+  : Lemma (to_i32x8 (from_i32x8 x) i == x i) 
+    [SMTPat (to_i32x8 (from_i32x8 x) i)] = admit ()
+
+let to_from_i32x8' (x: fnarr 8 i32)
+  : Lemma (to_i32x8 (from_i32x8 x) == x) 
+    [SMTPat (to_i32x8 (from_i32x8 x))]= admit ()
+
+assume val spec: i32 -> i32 -> i32
+
+let body (lhs rhs: bv): fnarr 8 i32 =
+  (FStar.FunctionalExtensionality.on_domain (i:
+        nat { i < 8 })
+      (fun i ->
+          match i with
+          | 0 -> spec (to_i32x8 lhs 0) (to_i32x8 rhs 0)
+          | 1 -> spec (to_i32x8 lhs 1) (to_i32x8 rhs 1)
+          | 2 -> spec (to_i32x8 lhs 2) (to_i32x8 rhs 2)
+          | 3 -> spec (to_i32x8 lhs 3) (to_i32x8 rhs 3)
+          | 4 -> spec (to_i32x8 lhs 4) (to_i32x8 rhs 4)
+          | 5 -> spec (to_i32x8 lhs 5) (to_i32x8 rhs 5)
+          | 6 -> spec (to_i32x8 lhs 6) (to_i32x8 rhs 6)
+          | 7 -> spec (to_i32x8 lhs 7) (to_i32x8 rhs 7)))
+
+unfold let test (lhs rhs: bv) = from_i32x8 (body lhs rhs)
+
+let test_lemma (lhs rhs: bv) =
+    // to_from_i32x8 (body lhs rhs) 0;
+    assert (
+        to_i32x8 (test lhs rhs) 0
+     == spec (to_i32x8 lhs 0) (to_i32x8 rhs 0)
+    )
